
\documentclass[11pt]{article}

\usepackage{fullpage}
\usepackage{amsmath}
\usepackage{amssymb}

\def\F#1#2{\mathtt{Float[#1,#2]}}

\begin{document}



$$
\frac{\mathsf{ufp}(\texttt{c})=u}
     {\Gamma \vdash \texttt{c\#p}\ :\ \F{u}{p} }
\hspace{2cm}
\frac{x : \F{u}{p} \in \Gamma}
     {\Gamma \vdash x\ :\ \F{u}{p} }
$$

$$\small
\begin{array}{c}
\texttt{+} : \Pi u_1:\texttt{int}. \Pi p_1:\texttt{int}.\Pi u_2:\texttt{int}. \Pi p_2:\texttt{int}.\\
\quad\F{u_1}{p_1}\rightarrow\F{u_2}{p_2}\rightarrow\F{u_1+u_2+1}{u_1+u_2+1-\max\big(\mathtt{u_1}-\mathtt{p_1},\mathtt{u_2}-\mathtt{p_2}\big)
-\iota\big(\mathtt{u_1}-\mathtt{p_1},\mathtt{u_2}-\mathtt{p_2}\big)
}
\end{array}
$$

$$\small
\begin{array}{l}
\texttt{+} : \Pi \mathtt{u_1}:\texttt{int}, \mathtt{p_1}:\texttt{int}, \mathtt{u_2}:\texttt{int}, \mathtt{p_2}:\texttt{int}.\\
\hspace{1.5cm}\F{u_1}{p_1}\rightarrow\F{u_2}{p_2}\rightarrow\F{\mathcal{U}_+(\mathtt{u_1},\mathtt{u_2})}{\mathcal{P}_+(\mathtt{u_1},\mathtt{u_2})}
\end{array}
$$


$$
\frac{\Gamma,x: \mathsf{T}_1 \vdash e :  \mathsf{T}_2}
     {\Gamma \vdash \lambda x:\mathsf{T}_1.e : \Pi x:\mathsf{T}_1 .  \mathsf{T}_2}
\hspace{2cm}
\frac{\Gamma \vdash e_1 : \Pi x: \mathsf{T}_1. \mathsf{T}_2\hspace{1cm} \Gamma \vdash e_2 :  \mathsf{T}_1}
     {\Gamma \vdash e_1\ e_2 :  \mathsf{T}_2[x\mapsto e_2]}
$$

\end{document}
